@prefix core: <http://kg.scania.com/core/> .
@prefix owl: <http://www.w3.org/2002/07/owl#> .
@prefix rdf: <http://www.w3.org/1999/02/22-rdf-syntax-ns#> .
@prefix rdfs: <http://www.w3.org/2000/01/rdf-schema#> .
@prefix xsd: <http://www.w3.org/2001/XMLSchema#> .
@prefix skos: <http://www.w3.org/2004/02/skos/core#> .

core:Metadata
  rdf:type owl:Class ;
  rdfs:comment "Metadata of the graph."@en ;
  rdfs:label "Metadata"@en ;
  core:timestamp "2023-11-27T15:25:00"^^xsd:dateTime .

core:contributor
  rdf:type owl:DatatypeProperty ;
  rdfs:comment "Contributor of the graph. Refers to the e-mail of contributor using the mailto-schema as of RFC 2368."@en ;
  rdfs:domain core:Metadata ;
  rdfs:label "contributor"@en ;
  rdfs:range xsd:string ;
  core:timestamp "2023-11-27T15:25:00"^^xsd:dateTime .

core:creator
  rdf:type owl:DatatypeProperty ;
  rdfs:comment "Creator of the graph. Refers to the e-mail of creator using the mailto-schema as of RFC 2368."@en ;
  rdfs:domain core:Metadata ;
  rdfs:label "creator"@en ;
  rdfs:range xsd:string ;
  core:timestamp "2023-11-27T15:25:00"^^xsd:dateTime .

core:graphType
  rdf:type owl:DatatypeProperty ;
  rdfs:comment "Access type of the graph. Refers to either SEMIPUBLIC, PUBLIC or PRIVATE string value."@en ;
  rdfs:domain core:Metadata ;
  rdfs:label "graph type"@en ;
  rdfs:range [
      rdf:type rdfs:Datatype ;
      owl:oneOf (
          "SEMIPUBLIC"
          "PRIVATE"
          "PUBLIC"
        ) ;
    ] ;
  core:timestamp "2023-11-27T15:25:00"^^xsd:dateTime .

core:informationResponsible
  rdf:type owl:DatatypeProperty ;
  rdfs:comment "Information responsible of the graph. Refers to the e-mail of information responsible using the mailto-schema as of RFC 2368."@en ;
  rdfs:domain core:Metadata ;
  rdfs:label "information responsible"@en ;
  rdfs:range xsd:string ;
  core:timestamp "2023-11-27T15:25:00"^^xsd:dateTime .

core:timestamp
  rdf:type owl:DatatypeProperty ;
  rdfs:comment "A point or period of time associated with an event in the lifecycle of the resource."@en ;
  rdfs:domain rdfs:Resource ;
  rdfs:label "timestamp"@en ;
  rdfs:range xsd:dateTime ;
  skos:scopeNote "To be reviewed and potentially replaced by more granular properties like dct:modified and dct:created" ;
  core:timestamp "2023-01-31T13:25:00"^^xsd:dateTime .

