@prefix core: <http://kg.scania.com/core/> .
@prefix owl: <http://www.w3.org/2002/07/owl#> .
@prefix rdf: <http://www.w3.org/1999/02/22-rdf-syntax-ns#> .
@prefix rdfs: <http://www.w3.org/2000/01/rdf-schema#> .
@prefix xsd: <http://www.w3.org/2001/XMLSchema#> .

core:Metadata
  rdf:type owl:Class ;
  rdfs:comment "Metadata of a knowledge graph or any other object."@en ;
  rdfs:label "Metadata"@en ;
  core:timestamp "2023-11-27T15:25:00"^^xsd:dateTime .

core:contributor
  rdf:type owl:DatatypeProperty ;
  rdfs:comment "Contributor to the ontology. Refers to the e-mail of contributor using the mailto-schema as of RFC 2368."@en ;
  rdfs:domain core:Metadata ;
  rdfs:label "contributor"@en ;
  rdfs:range xsd:string ;
  core:timestamp "2023-11-27T15:25:00"^^xsd:dateTime .

core:creator
  rdf:type owl:DatatypeProperty ;
  rdfs:comment "Creator of the ontology. Refers to the e-mail of creator using the mailto-schema as of RFC 2368."@en ;
  rdfs:domain core:Metadata ;
  rdfs:label "creator"@en ;
  rdfs:range xsd:string ;
  core:timestamp "2023-11-27T15:25:00"^^xsd:dateTime .

core:graphType
  rdf:type owl:DatatypeProperty ;
  rdfs:comment "Graph type of the ontology. Refers to either SEMIPUBLIC, PUBLIC or PRIVATE string value."@en ;
  rdfs:domain core:Metadata ;
  rdfs:label "graph type"@en ;
  rdfs:range [
      rdf:type rdfs:Datatype ;
      owl:oneOf (
          "SEMIPUBLIC"
          "PRIVATE"
          "PUBLIC"
        ) ;
    ] ;
  core:timestamp "2023-11-27T15:25:00"^^xsd:dateTime .

core:informationResponsible
  rdf:type owl:DatatypeProperty ;
  rdfs:comment "Information responsible of the ontology is in charge of approving the ontology (being reviewed) from a business point of view. Refers to the e-mail of information responsible using the mailto-schema as of RFC 2368."@en ;
  rdfs:domain core:Metadata ;
  rdfs:label "information responsible"@en ;
  rdfs:range xsd:string ;
  core:timestamp "2023-11-27T15:25:00"^^xsd:dateTime .
